Spqr/Specs/Encoding/Polynomial/Pt/Deserialize.lean
@@ -150,19 +150,9 @@ theorem deserialize_spec (s : Array Std.U8 4#usize) :
   unfold deserialize encoding.gf.GF16.new core.result.Result.unwrap
   step*
   simp_all only
-  split
-  · -- `try_from` on `s[0..2]` returned `Ok`
-    simp_all only
-    step*
-    simp_all only
-    split
-    · -- `try_from` on `s[2..4]` returned `Ok`
-      simp_all only
-      step*
-      simp_all
-    · -- `try_from` on `s[2..4]` returned `Err`: contradiction
-      simp_all
-  · -- `try_from` on `s[0..2]` returned `Err`: contradiction
-    simp_all
+  step*
+  simp_all only
+  step*
+  simp_all
 
 end spqr.encoding.polynomial.Pt
